WIP on Ethernet Frames.

src/BinEncoders/Env/Examples/EthernetFrame.v
@@ -3,7 +3,6 @@ Require Import
         Coq.Vectors.Vector.
 
 Require Import
-        Fiat.Examples.DnsServer.Packet
         Fiat.Common.SumType
         Fiat.Common.BoundedLookup
         Fiat.Common.ilist
@@ -16,19 +15,20 @@ Require Import
         Fiat.BinEncoders.Env.Common.Compose
         Fiat.BinEncoders.Env.Common.ComposeOpt
         Fiat.BinEncoders.Env.Automation.Solver
+        Fiat.BinEncoders.Env.Lib2.FixListOpt
+        Fiat.BinEncoders.Env.Lib2.NoCache
         Fiat.BinEncoders.Env.Lib2.WordOpt
         Fiat.BinEncoders.Env.Lib2.NatOpt
-        Fiat.BinEncoders.Env.Lib2.StringOpt
+        Fiat.BinEncoders.Env.Lib2.Vector
         Fiat.BinEncoders.Env.Lib2.EnumOpt
-        Fiat.BinEncoders.Env.Lib2.FixListOpt
-        Fiat.BinEncoders.Env.Lib2.SumTypeOpt
-        Fiat.BinEncoders.Env.Lib2.DomainNameOpt.
+        Fiat.BinEncoders.Env.Lib2.SumTypeOpt.
 
 Require Import
         Bedrock.Word.
 
 Import Vectors.VectorDef.VectorNotations.
 Open Scope string_scope.
+Open Scope Tuple_scope.
 
 Definition EthernetFrame :=
   @Tuple <"Destination" :: Vector.t char 6,
@@ -36,20 +36,474 @@ Definition EthernetFrame :=
           "Type" :: BoundedString ["ARP"; "IP"; "RARP"],
           "Data" :: list char>.
 
-  Definition EthernetFrame_Spec (p : EthernetFrame) :=
-       encode_word_Spec p!"id"
-  Then encode_word_Spec (WS p!"QR" WO)
-  Then encode_enum_Spec Opcode_Ws p!"Opcode"
-  Then encode_word_Spec (WS p!"AA" WO)
-  Then encode_word_Spec (WS p!"TC" WO)
-  Then encode_word_Spec (WS p!"RD" WO)
-  Then encode_word_Spec (WS p!"RA" WO)
-  Then encode_word_Spec (WS false (WS false (WS false WO))) (* 3 bits reserved for future use *)
-  Then encode_enum_Spec RCODE_Ws p!"RCODE"
-  Then encode_nat_Spec 16 1 (* length of question field *)
-  Then encode_nat_Spec 16 (|p!"answers"|)
-  Then encode_nat_Spec 16 (|p!"authority"|)
-  Then encode_nat_Spec 16 (|p!"additional"|)
-  Then encode_question_Spec p!"question"
-  Then (encode_list_Spec encode_resource_Spec (p!"answers" ++ p!"additional" ++ p!"authority"))
-  Done.
+Definition EtherTypeCodes : Vector.t (word 16) 3 :=
+  [WO~0~0~0~0~0~0~0~0~0~0~0~1~0~0~0~0;
+   WO~0~1~1~0~0~0~0~0~0~0~0~1~0~0~0~0;
+   WO~1~0~1~0~1~1~0~0~0~0~0~1~0~0~0~0
+  ].
+
+  Definition transformer : Transformer ByteString := ByteStringTransformer.
+
+  Local Notation "x ++ y" := (transform x y).
+
+Definition composeIf E B
+           (transformer : Transformer B)
+           (encode1 : E -> Comp (B * E))
+           (iComp : Comp bool)
+           (encodeT : E -> Comp (B * E))
+           (encodeE : E -> Comp (B * E))
+  :=
+  (fun e0 =>
+     `(p, e1) <- encode1 e0;
+       b <- iComp;
+       If b Then
+          `(q, e2) <- encodeT e1;
+          ret (transform p q, e2)
+       Else (`(q, e2) <- encodeE e1;
+            ret (transform p q, e2))
+  )%comp.
+
+Lemma composeIf_encode_correct
+      {A A' B}
+      {cache : Cache}
+      {P  : CacheDecode -> Prop}
+      {P_inv1 P_invT P_invE : (CacheDecode -> Prop) -> Prop}
+      (P_inv_pf : cache_inv_Property P (fun P => P_inv1 P /\ P_invT P /\ P_invE P))
+      (transformer : Transformer B)
+      (project : A -> A')
+      (predicate : A -> Prop)
+      (predicate_rest : A' -> B -> Prop)
+      (predicate_rest' : A -> B -> Prop)
+      (predicate' : A' -> Prop)
+      (encode1 : A' -> CacheEncode -> Comp (B * CacheEncode))
+      (decode1 : B -> CacheDecode -> option (A' * B * CacheDecode))
+      (IComp : Comp bool)
+      (ICompb : A' -> B -> bool)
+      (encodeT : A -> CacheEncode -> Comp (B * CacheEncode))
+      (decodeT : A' -> B -> CacheDecode -> option (A * B * CacheDecode))
+      (encodeE : A -> CacheEncode -> Comp (B * CacheEncode))
+      (decodeE : A' -> B -> CacheDecode -> option (A * B * CacheDecode))
+      (decode1_pf :
+         cache_inv_Property P P_inv1
+         -> encode_decode_correct_f
+              cache transformer predicate' predicate_rest
+              encode1 decode1 P)
+      (decodeT_pf : forall proj,
+          IComp true ->
+          predicate' proj ->
+          cache_inv_Property P P_invT ->
+          encode_decode_correct_f
+            cache transformer
+            (fun data => predicate data /\ project data = proj)
+            predicate_rest'
+            encodeT
+            (decodeT proj) P)
+      (decodeE_pf : forall proj,
+          IComp false ->
+          predicate' proj ->
+          cache_inv_Property P P_invE ->
+          encode_decode_correct_f
+            cache transformer
+            (fun data => predicate data /\ project data = proj)
+            predicate_rest'
+            encodeE
+            (decodeE proj) P)
+      (ICompb_decT :
+         forall data env b b' c xenv ext,
+           predicate data
+           -> encode1 (project data) env ↝ (b, c)
+           -> IComp ↝ true
+           -> encodeT data c ↝ (b', xenv)
+           -> ICompb (project data) (transform b' ext) = true)
+      (ICompb_decE :
+         forall data env b b' c xenv ext,
+           predicate data
+           -> encode1 (project data) env ↝ (b, c)
+           -> IComp ↝ false
+           -> encodeE data c ↝ (b', xenv)
+           -> ICompb (project data) (transform b' ext) = false)
+      (ICompb_dec :
+         forall a b,
+           IComp (ICompb a b))
+      (predicate_rest_implT : forall a' b b'',
+          (IComp true /\
+          exists a ce ce' ce'' b' b'',
+            computes_to (encode1 a' ce) (b', ce')
+            /\ project a = a'
+            /\ predicate a
+            /\ computes_to (encodeT a ce') (b'', ce'')
+            /\ predicate_rest' a b)
+          -> predicate_rest a' (transform b'' b))
+      (predicate_rest_implE : forall a' b b'',
+          (IComp false /\
+          exists a ce ce' ce'' b',
+            computes_to (encode1 a' ce) (b', ce')
+            /\ project a = a'
+            /\ predicate a
+            /\ computes_to (encodeE a ce') (b'', ce'')
+            /\ predicate_rest' a b)
+          -> predicate_rest a' (transform b'' b))
+      (pred_pf : forall data, predicate data -> predicate' (project data))      
+  : encode_decode_correct_f
+      cache transformer
+      (fun a => predicate a)
+      predicate_rest'
+      (fun (data : A) (ctx : CacheEncode) =>
+         composeIf _ _ _ (encode1 (project data)) IComp (encodeT data) (encodeE data)  ctx
+      )%comp
+     (fun (bin : B) (env : CacheDecode) =>
+        `(proj, rest, env') <- decode1 bin env;
+          If (ICompb proj) rest Then
+             decodeT proj rest env'
+             Else
+             decodeE proj rest env'
+     ) P.
+Proof.
+  unfold cache_inv_Property in *; split.
+  { intros env env' xenv data bin ext env_pm pred_pm pred_pm_rest com_pf.
+    unfold composeIf, Bind2 in com_pf; computes_to_inv; destruct v;
+      destruct v0; simpl in com_pf''.
+    - computes_to_inv; destruct v; subst.
+      destruct (fun H => proj1 (decode1_pf (proj1 P_inv_pf)) _ _ _ _ _ (transform b0 ext) env_pm (pred_pf _ pred_pm) H com_pf); intuition; simpl in *; injections.
+      eapply predicate_rest_implT; repeat eexists; intuition eauto.
+      pose proof (ICompb_decT _ _ _ _ _ _ ext pred_pm com_pf com_pf' com_pf'').
+      destruct (fun H' => proj1 (decodeT_pf (project data) com_pf' (pred_pf _ pred_pm)
+                                  H)
+                      _ _ _ _ _ ext H3 (conj pred_pm (eq_refl _)) H' com_pf'');
+        intuition; simpl in *; injections.
+      setoid_rewrite <- transform_assoc; rewrite H2.
+      intuition; simpl in *; injections.
+      rewrite H5, H7; simpl; eauto.
+    - computes_to_inv; destruct v; subst.
+      destruct (fun H' => proj1 (decode1_pf (proj1 P_inv_pf)) _ _ _ _ _ (transform b0 ext) env_pm (pred_pf _ pred_pm) H' com_pf); intuition; simpl in *; injections.
+      eapply predicate_rest_implE; intuition; repeat eexists; intuition eauto.
+      pose proof (ICompb_decE _ _ _ _ _ _ ext pred_pm com_pf com_pf' com_pf'').
+      destruct (fun H' => proj1 (decodeE_pf (project data) com_pf' (pred_pf _ pred_pm)
+                                  H4)
+                      _ _ _ _ _ ext H3 (conj pred_pm (eq_refl _)) H' com_pf'');
+        intuition; simpl in *; injections.
+      setoid_rewrite <- transform_assoc; rewrite H2.
+      intuition; simpl in *; injections.
+      rewrite H5, H7; simpl; eauto.
+  }
+  { intros.
+    destruct (decode1 bin env') as [ [ [? ?] ? ] | ] eqn : ? ;
+      simpl in *; try discriminate.
+    pose proof (ICompb_dec a b) as ICompb'.
+    destruct (ICompb a b) eqn: ?; simpl in *.
+    - eapply (proj2 (decode1_pf (proj1 P_inv_pf))) in Heqo; eauto;
+        destruct Heqo; destruct_ex; intuition;
+          eapply (proj2 (decodeT_pf a ICompb' H7 H3)) in H1; eauto;
+            destruct H1; destruct_ex; intuition; subst.
+      eexists; eexists; repeat split.
+      repeat computes_to_econstructor; eauto.
+      simpl; repeat computes_to_econstructor; eauto.
+      simpl; rewrite transform_assoc; reflexivity.
+      eassumption.
+      eassumption.
+    - eapply (proj2 (decode1_pf (proj1 P_inv_pf))) in Heqo; eauto;
+        destruct Heqo; destruct_ex; intuition;
+          eapply (proj2 (decodeE_pf a ICompb' H7 H8)) in H1; eauto;
+            destruct H1; destruct_ex; intuition; subst.
+      eexists; eexists; repeat split.
+      repeat computes_to_econstructor; eauto.
+      simpl; repeat computes_to_econstructor; eauto.
+      simpl; rewrite transform_assoc; reflexivity.
+      eassumption.
+      eassumption.
+  }
+Qed.
+
+Local Notation "x 'ThenIf' i 'TheniC' t 'ElseiC' e " :=
+  (composeIf _ _ _ x i t e) (at level 100, right associativity).
+
+  Definition encode_EthernetFrame_Spec (eth : EthernetFrame) :=
+      (encode_Vector_Spec encode_word_Spec eth!"Destination")
+        ThenC (encode_Vector_Spec encode_word_Spec eth!"Source")
+        ThenIf ({v1042 : bool | True}) (* Support both kinds of frames.*)
+        TheniC
+        (encode_nat_Spec 16 (length eth!"Data")
+           ThenC encode_word_Spec (WO~0~1~0~1~0~1~0~1)
+           ThenC encode_word_Spec (WO~0~1~0~1~0~1~0~1)
+           ThenC encode_word_Spec (WO~1~1~0~0~0~0~0~0)
+           ThenC encode_word_Spec (wzero 24)
+           ThenC encode_enum_Spec EtherTypeCodes eth!"Type"
+           ThenC encode_list_Spec encode_word_Spec eth!"Data"
+           DoneC)
+       ElseiC
+       encode_enum_Spec EtherTypeCodes eth!"Type"
+       ThenC encode_list_Spec encode_word_Spec eth!"Data"
+       DoneC.
+
+  Opaque pow2. (* Don't want to be evaluating this. *)
+
+  Ltac apply_compose :=
+    intros;
+    match goal with
+      H : cache_inv_Property ?P ?P_inv |- _ =>
+      first [eapply (compose_encode_correct_no_dep H); clear H
+            | eapply (compose_encode_correct H); clear H
+            | eapply (composeIf_encode_correct H); clear H
+            ]
+    end.
+
+  Ltac makeEvar T k :=
+    let x := fresh in evar (x : T); let y := eval unfold x in x in clear x; k y.
+
+  Ltac shelve_inv :=
+    let H' := fresh in
+    let data := fresh in
+    intros data H';
+    repeat destruct H';
+    match goal with
+    | H : ?P data |- ?P_inv' =>
+      is_evar P;
+      let P_inv' := (eval pattern data in P_inv') in
+      let P_inv := match P_inv' with ?P_inv data => P_inv end in
+      let new_P_T := type of P in
+      makeEvar new_P_T
+               ltac:(fun new_P =>
+                       unify P (fun data => new_P data /\ P_inv data)); apply (Logic.proj2 H)
+    end.    
+  
+  Theorem decode_list_all_correct_ComposeOpt
+      : encode_decode_correct_f
+          _ transformer
+          (fun a => True)
+          (fun _ b => b = transform_id)
+          (encode_list_Spec encode_word_Spec)
+          (fun (bin : ByteString) (env : CacheDecode) =>
+             Some (byteString bin, ByteString_id, tt))
+          (fun a => True).
+  Proof.
+    split.
+    {
+      intros env env' xenv l l' ext Eeq Ppred Ppred_rest Penc.
+      intuition; subst.
+      generalize dependent env. generalize dependent env'.
+      generalize dependent xenv.
+      generalize dependent l'. induction l.
+      { intros.
+        simpl in *; intuition; computes_to_inv;
+          injections; simpl.
+        eexists; eauto. }
+      { intros; simpl in *.
+        unfold Bind2 in Penc; computes_to_inv; subst.
+        destruct v; destruct v0; simpl in *.
+        injections.
+        eapply IHl in Penc'; eauto.
+        destruct_ex; intuition; injections.
+        pose proof transform_assoc;
+          pose proof transform_id_right.
+        simpl in H, H0.
+        setoid_rewrite <- H.
+        setoid_rewrite H0; eexists; intuition; repeat f_equal.
+        unfold encode_word_Spec in Penc.
+        simpl in Penc.
+        admit.
+      }
+    }
+    { admit.
+    }
+  Qed.
+
+  Ltac solve_data_inv :=
+    first [ simpl; intros; exact I
+          | shelve_inv ].
+
+  Lemma Vector_predicate_rest_True n
+    : forall a' b,
+      Vector_predicate_rest (fun (_ : word 8) (_ : ByteString) => True) encode_word_Spec n a' b.
+  Proof.
+    induction a'; simpl; eauto.
+  Qed.
+
+  Ltac finalize_decoder P_inv :=
+  (unfold encode_decode_correct_f; intuition eauto);
+    [ computes_to_inv; injections; subst; simpl;
+      match goal with
+        H : Equiv _ ?env |- _ =>
+        eexists env; intuition eauto;
+        simpl;
+        match goal with
+          |- ?f ?a ?b ?c = ?P =>
+          let P' := (eval pattern a, b, c in P) in
+          let f' := match P' with ?f a b c => f end in
+          unify f f'; reflexivity
+        end
+      end
+    | injections; eauto
+    | eexists _; eexists _;
+      intuition eauto; injections; eauto using idx_ibound_eq;
+      try match goal with
+        |- P_inv ?data => destruct data;
+                                 simpl in *; eauto
+      end
+    ].
+
+  Lemma Check_Integrity {A B C D E F}
+        (b_eq_dec : forall b', DecideableEnsembles.DecideableEnsemble (fun b : B => b = b'))
+    : forall (a a' : A) (f : A -> B) (b : B) (f' : A -> C -> D -> option F) f'' (c : C) (d : D) (e : E) (P : E -> E -> Prop),
+      a = a'
+      -> f a = b
+      -> (exists e' : E,
+          f' a' c d = Some (f'' e') /\ P e e')
+      -> exists e' : E,
+          If DecideableEnsembles.dec (DecideableEnsemble := b_eq_dec b) (f a') Then f' a' c d Else None = Some (f'' e') /\ P e e'.
+  Proof.
+    intros.
+    rewrite H in H0.
+    intros; apply (DecideableEnsembles.dec_decides_P (DecideableEnsemble := b_eq_dec b)) in H0.
+    rewrite H0; simpl; intros; eauto.
+  Qed.        
+
+  Global Instance Query_eq_nat : DecideableEnsembles.Query_eq nat :=
+    {| A_eq_dec := Coq.Arith.Peano_dec.eq_nat_dec |}.
+
+  Definition packet_decoder
+    : { decodePlusCacheInv |
+        exists P_inv pred,
+        (cache_inv_Property (snd decodePlusCacheInv) P_inv
+        -> encode_decode_correct_f _ transformer pred (fun _ b => b = ByteString_id) encode_EthernetFrame_Spec (fst decodePlusCacheInv) (snd decodePlusCacheInv))
+        /\ cache_inv_Property (snd decodePlusCacheInv) P_inv}.
+  Proof.
+    eexists (_, _); eexists _; eexists _; split; simpl.
+    intros.
+    apply_compose.
+    intro. eapply Vector_decode_correct.
+    revert H; eapply Word_decode_correct.
+    solve_data_inv.
+    intros; apply Vector_predicate_rest_True.
+    apply_compose.
+    intro. eapply Vector_decode_correct.
+    revert H0; eapply Word_decode_correct.
+    apply_compose.
+    eapply Nat_decode_correct.
+    solve_data_inv.
+    simpl; intros; exact I.
+    apply_compose.
+    eapply Word_decode_correct.
+    solve_data_inv.
+    simpl; intros; exact I.
+    apply_compose.
+    eapply Word_decode_correct.
+    solve_data_inv.
+    simpl; intros; exact I.
+    apply_compose.
+    eapply Word_decode_correct.
+    solve_data_inv.
+    simpl; intros; exact I.
+    apply_compose.
+    eapply Word_decode_correct.
+    solve_data_inv.
+    simpl; intros; exact I.
+    apply_compose.
+    eapply Enum_decode_correct.
+    admit.
+    solve_data_inv.
+    simpl; intros; exact I.
+    apply_compose.
+    intros; eapply decode_list_all_correct_ComposeOpt.
+    solve_data_inv.
+    simpl; intros.
+    computes_to_inv; injections.
+    pose proof transform_id_left as H'; simpl in H'; rewrite H'; reflexivity.
+    simpl; intros.
+    unfold encode_decode_correct_f; intuition eauto.
+    match goal with
+      [H : ?p = ?proj1, H2 : ?f ?p = ?proj2 |-
+       exists xenv', ?f' ?proj1 ?b ?env' = Some (?data, ?ext, xenv') /\ Equiv xenv xenv'] =>
+      instantiate (1 := fun p b' c => if (DecideableEnsembles.A_eq_dec (f p) proj2) then _ p b' c else None); cbv beta
+    end.
+    destruct (@DecideableEnsembles.A_eq_dec nat Query_eq_nat 
+               (@Datatypes.length char proj3) proj1); try congruence. 
+    destruct data as [? [? [? [? [ ] ] ] ] ]; 
+      unfold GetAttribute, GetAttributeRaw in *;
+      simpl in *.
+    computes_to_inv; injections; subst; simpl.
+    pose proof transform_id_left as H'; simpl in H'; rewrite H'.
+    eexists tt; simpl; intuition eauto.
+    match goal with
+      |- ?f ?a ?b ?c = ?P =>
+      let P' := (eval pattern a, b, c in P) in
+      let f' := match P' with ?f a b c => f end in
+      try unify f f'; try reflexivity
+    end.
+    cbv beta in H12.
+    destruct (@DecideableEnsembles.A_eq_dec nat Query_eq_nat 
+                                              (@Datatypes.length char proj3) proj1); try congruence; subst.
+    eexists _; eexists tt;
+      intuition eauto; injections; eauto using idx_ibound_eq;
+        try match goal with
+              |-  ?data => destruct data;
+                             simpl in *; eauto
+            end.
+    destruct env; computes_to_econstructor.
+    pose proof transform_id_left as H'; simpl in H'; rewrite H'.
+    reflexivity.
+    Focus 2.
+    apply_compose.
+    eapply Enum_decode_correct.
+    admit.
+    solve_data_inv.
+    simpl; intros; exact I.
+    apply_compose.
+    intros; eapply decode_list_all_correct_ComposeOpt.
+    solve_data_inv.
+    simpl; intros.
+    computes_to_inv; injections.
+    pose proof transform_id_left as H'; simpl in H'; rewrite H'; reflexivity.
+    simpl; intros.
+    unfold encode_decode_correct_f; intuition eauto.
+    destruct data as [? [? [? [? [ ] ] ] ] ]; 
+      unfold GetAttribute, GetAttributeRaw in *;
+      simpl in *.
+    computes_to_inv; injections; subst; simpl.
+    pose proof transform_id_left as H'; simpl in H'; rewrite H'.
+    eexists tt; simpl; intuition eauto.
+    match goal with
+      |- ?f ?a ?b ?c = ?P =>
+      let P' := (eval pattern a, b, c in P) in
+      let f' := match P' with ?f a b c => f end in
+      try unify f f'; try reflexivity
+    end.
+    eexists _; eexists tt;
+      intuition eauto; injections; eauto using idx_ibound_eq;
+        try match goal with
+              |-  ?data => destruct data;
+                             simpl in *; eauto
+            end.
+    destruct env; computes_to_econstructor.
+    pose proof transform_id_left as H'; simpl in H'; rewrite H'.
+    reflexivity.
+
+
+    
+
+        intros; eapply FixList_decode_correct.
+    revert H8; eapply Word_decode_correct.
+    solve_data_inv.
+    unfold encode_decode_correct_f.
+
+    let H' := fresh in
+    let data := fresh in
+    let H'' := fresh in
+    intros H' data H'';
+    repeat destruct H'';
+    match goal with
+    | H : ?P data |- ?P_inv' =>
+      is_evar P;
+        let P_inv' := (eval pattern data in P_inv') in
+        let P_inv := match P_inv' with ?P_inv data => P_inv end in
+        let new_P_T := type of P in
+        makeEvar new_P_T
+                 ltac:(fun new_P =>
+                         try unify P (fun data => new_P data /\ P_inv data)); try apply (Logic.proj2 H)
+    end.
+
+    shelve_inv.
+    split.
+    intros.
+    unfold encode_EthernetFrame_Spec in H2.
+    unfold compose, Bind2 in H2; computes_to_inv.
+    computes_to_inv.
