src/BinEncoders/Env/Lib2/Vector.v
@@ -14,10 +14,14 @@ Section Vector.
   Context {transformer : Transformer B}.
 
   Variable A_predicate : A -> Prop.
+  Variable A_predicate_rest : A -> B -> Prop.
   Variable A_encode_Spec : A -> CacheEncode -> Comp (B * CacheEncode).
   Variable A_decode : B -> CacheDecode -> option (A * B * CacheDecode).
   Variable A_cache_inv : CacheDecode -> Prop.
-  Variable A_decode_pf : encode_decode_correct_f cache transformer A_predicate A_encode_Spec A_decode A_cache_inv.
+  Variable A_decode_pf
+    : encode_decode_correct_f cache transformer A_predicate
+                              A_predicate_rest
+                              A_encode_Spec A_decode A_cache_inv.
 
   Fixpoint encode_Vector_Spec {n} (xs : Vector.t A n) (ce : CacheEncode)
     : Comp (B * CacheEncode) :=
@@ -49,34 +53,74 @@ Section Vector.
               Some (Vector.cons _ x _ xs, b2, e2)
     end.
 
-  Theorem FixVector_decode_correct
+(*  Lemma Vector_encode_preserves_rest_predicate
+    : forall (sz : nat)
+             (l : Vector.t A sz)
+             (ext : B)
+             (env xenv : CacheEncode) (l' : B) a a',
+      encode_Vector_Spec l env ↝ (l', xenv) ->
+      (forall x : A, Vector.In x l -> A_predicate x) ->
+      A_predicate_rest a ext ->
+      A_predicate_rest a' (transform l' ext).
+  Proof.
+    induction l.
+    - simpl in *; intuition; computes_to_inv;
+        injections; simpl; rewrite transform_id_left; eauto.
+    - intros; simpl in *.
+      unfold Bind2 in H; computes_to_inv; subst.
+      destruct v; destruct v0; simpl in *.
+      injections.
+      rewrite <- transform_assoc.
+      eapply A_predicate_rest_inv; eauto.
+      eapply H0; econstructor.
+      eapply (IHl _ _ _ _ _ H' (fun x H'' => H0 x (Vector.In_cons_tl _ _ _ H''))); intuition eauto.
+  Qed. *)
+
+  Fixpoint Vector_predicate_rest
+           n
+           (As : Vector.t A n)
+           (b : B)
+    : Prop :=
+    match As with
+    | Vector.nil => True
+    | Vector.cons a _ As' =>
+      (forall b' ce ce',
+          computes_to (encode_Vector_Spec As' ce) (b', ce')
+          -> A_predicate_rest a (transform b' b))
+      /\ Vector_predicate_rest _ As' b
+    end.
+
+  Theorem Vector_decode_correct
     :
     forall sz,
       encode_decode_correct_f
         cache transformer
         (fun ls => forall x, Vector.In x ls -> A_predicate x)
+        (Vector_predicate_rest sz)
         encode_Vector_Spec (decode_Vector sz) A_cache_inv.
   Proof.
     split.
     {
-      intros env env' xenv l l' ext Eeq Ppred Penc.
+      intros env env' xenv l l' ext Eeq Ppred Ppred_rest Penc.
       generalize dependent env. generalize dependent env'.
       generalize dependent xenv.
       generalize dependent l'. induction l.
       { intros.
         simpl in *; intuition; computes_to_inv;
-          injections; simpl.
-        rewrite transform_id_left; eexists; eauto. }
+          injections; simpl; rewrite transform_id_left; eauto.
+      }
       { intros; simpl in *.
         assert (A_predicate h) by (eapply Ppred; econstructor).
         unfold Bind2 in Penc; computes_to_inv; subst.
         destruct v; destruct v0; simpl in *.
         injections.
-        destruct (proj1 A_decode_pf _ _ _ _ _ (transform b0 ext) Eeq H Penc) as [ ? [? ?] ].
+        destruct (fun H' => proj1 A_decode_pf _ _ _ _ _ (transform b0 ext) Eeq H H' Penc) as [ ? [? ?] ].
+        intuition; destruct_ex.
+        eapply H0; eauto.
         setoid_rewrite <- transform_assoc; setoid_rewrite H0;
           simpl.
-        destruct (IHl (fun x H => Ppred x (Vector.In_cons_tl _ _ _ H)) b0 xenv x c); intuition eauto.
-        setoid_rewrite H3; simpl.
+        destruct (fun H' => IHl (fun x H => Ppred x (Vector.In_cons_tl _ _ _ H)) H' b0 xenv x c); intuition eauto.
+        setoid_rewrite H5; simpl.
         eexists; intuition.
       }
     }
@@ -89,8 +133,8 @@ Section Vector.
         destruct (decode_Vector sz b c) as [ [ [? ?] ?] | ] eqn: ? ;
           simpl in *; try discriminate; injections.
         eapply (proj2 A_decode_pf) in Heqo; eauto;
-          destruct Heqo; destruct_ex; intuition; subst;
-            eapply IHsz in Heqo0; eauto; destruct Heqo0;
+          destruct Heqo as [? [? ?] ]; destruct_ex; intuition; subst;
+            eapply IHsz in Heqo0; eauto; destruct Heqo0 as [? [? ?] ];
               destruct_ex; intuition; subst.
         simpl.
         eexists; eexists; intuition eauto.
