src/BinEncoders/Env/Common/ComposeOpt.v
@@ -14,8 +14,8 @@ Definition compose E B
     `(q, e2) <- encode2 e1;
     ret (transform p q, e2))%comp.
 
-Notation "x 'Then' y" := (compose _ x y) (at level 100, right associativity).
-Notation "x 'Done'"   := (x Then fun e => ret (transform_id, e)) (at level 99, right associativity).
+Notation "x 'ThenC' y" := (compose _ x y) (at level 100, right associativity).
+Notation "x 'DoneC'"   := (x ThenC fun e => ret (transform_id, e)) (at level 99, right associativity).
 
 Lemma refineEquiv_compose_compose E B
            (transformer : Transformer B)
@@ -77,24 +77,40 @@ Lemma compose_encode_correct
       (project : A -> A')
       (predicate : A -> Prop)
       (predicate' : A' -> Prop)
+      (predicate_rest' : A -> B -> Prop)
+      (predicate_rest : A' -> B -> Prop)
       (encode1 : A' -> CacheEncode -> Comp (B * CacheEncode))
       (encode2 : A -> CacheEncode -> Comp (B * CacheEncode))
       (decode1 : B -> CacheDecode -> option (A' * B * CacheDecode))
       (decode1_pf :
          cache_inv_Property P P_inv1
-         -> encode_decode_correct_f cache transformer predicate' encode1 decode1 P)
+         -> encode_decode_correct_f
+              cache transformer predicate'
+              predicate_rest
+              encode1 decode1 P)
       (pred_pf : forall data, predicate data -> predicate' (project data))
+      (predicate_rest_impl :
+         forall a' b
+                a ce ce' ce'' b' b'',
+           computes_to (encode1 a' ce) (b', ce')
+           -> project a = a'
+           -> predicate a
+           -> computes_to (encode2 a ce') (b'', ce'')
+           -> predicate_rest' a b
+          -> predicate_rest a' (transform b'' b))
       (decode2 : A' -> B -> CacheDecode -> option (A * B * CacheDecode))
       (decode2_pf : forall proj,
           predicate' proj ->
           cache_inv_Property P P_inv2 ->
           encode_decode_correct_f cache transformer
             (fun data => predicate data /\ project data = proj)
+            predicate_rest'
             encode2
             (decode2 proj) P)
   : encode_decode_correct_f
       cache transformer
       (fun a => predicate a)
+      predicate_rest'
       (fun (data : A) (ctx : CacheEncode) =>
          compose _ (encode1 (project data)) (encode2 data)  ctx
       )%comp
@@ -103,23 +119,24 @@ Lemma compose_encode_correct
           decode2 proj rest env') P.
 Proof.
   unfold cache_inv_Property in *; split.
-  { intros env env' xenv data bin ext env_pm pred_pm com_pf.
+  { intros env env' xenv data bin ext env_pm pred_pm pred_pm_rest com_pf.
     unfold compose, Bind2 in com_pf; computes_to_inv; destruct v;
       destruct v0.
-    destruct (proj1 (decode1_pf (proj1 P_inv_pf)) _ _ _ _ _ (transform b0 ext) env_pm (pred_pf _ pred_pm) com_pf); intuition; simpl in *; injections.
+    destruct (fun H' => proj1 (decode1_pf (proj1 P_inv_pf)) _ _ _ _ _ (transform b0 ext) env_pm (pred_pf _ pred_pm) H' com_pf); intuition; simpl in *; injections; eauto.
+
     setoid_rewrite <- transform_assoc; rewrite H2.
     simpl.
-    destruct (proj1 (decode2_pf (project data) (pred_pf _ pred_pm) H1)
-                    _ _ _ _ _ ext H3 (conj pred_pm (eq_refl _)) com_pf');
+    destruct (fun H'' => proj1 (decode2_pf (project data) (pred_pf _ pred_pm) H1)
+                               _ _ _ _ _ ext H3 (conj pred_pm (eq_refl _)) H'' com_pf');
       intuition; simpl in *; injections.
     eauto. }
   { intros.
     destruct (decode1 bin env') as [ [ [? ?] ? ] | ] eqn : ? ;
       simpl in *; try discriminate.
-    eapply (proj2 (decode1_pf (proj1 P_inv_pf))) in Heqo; eauto;
-      destruct Heqo; destruct_ex; intuition;
-        eapply (proj2 (decode2_pf a H7 H5)) in H1; eauto;
-          destruct H1; destruct_ex; intuition; subst.
+    eapply (proj2 (decode1_pf (proj1 P_inv_pf))) in Heqo; eauto.
+      destruct Heqo as [? [? [? [? [? [? ?] ] ] ] ] ].
+    eapply (proj2 (decode2_pf a H5 (proj2 P_inv_pf))) in H2; eauto.
+    destruct H2 as [? ?]; destruct_ex; intuition; subst.
     eexists; eexists; repeat split.
     repeat computes_to_econstructor; eauto.
     simpl; rewrite transform_assoc; reflexivity.
@@ -139,24 +156,37 @@ Lemma compose_encode_correct_no_dep
       (a' : A')
       (predicate : A -> Prop)
       (predicate' : A' -> Prop)
+      (predicate_rest' : A -> B -> Prop)
+      (predicate_rest : A' -> B -> Prop)
       (encode1 : A' -> CacheEncode -> Comp (B * CacheEncode))
       (encode2 : A -> CacheEncode -> Comp (B * CacheEncode))
       (decode1 : B -> CacheDecode -> option (A' * B * CacheDecode))
       (decode1_pf :
          cache_inv_Property P P_inv1
-         -> encode_decode_correct_f cache transformer predicate' encode1 decode1 P)
+         -> encode_decode_correct_f cache transformer predicate' predicate_rest
+                                    encode1 decode1 P)
       (predicate_a' : predicate' a')
+      (predicate_rest_impl :
+         forall a' b
+                a ce ce' ce'' b' b'',
+           computes_to (encode1 a' ce) (b', ce')
+           -> predicate a
+           -> computes_to (encode2 a ce') (b'', ce'')
+           -> predicate_rest' a b
+           -> predicate_rest a' (transform b'' b))
       (decode2 : B -> CacheDecode -> option (A * B * CacheDecode))
       (decode2_pf :
          predicate' a' ->
           cache_inv_Property P P_inv2 ->
           encode_decode_correct_f cache transformer
-            (fun data => predicate data)
+                                  (fun data => predicate data)
+                                  predicate_rest'
             encode2
             decode2 P)
   : encode_decode_correct_f
       cache transformer
       (fun a => predicate a)
+      predicate_rest'
       (fun (data : A) (ctx : CacheEncode) =>
          compose _ (encode1 a') (encode2 data)  ctx
       )%comp
@@ -165,16 +195,17 @@ Lemma compose_encode_correct_no_dep
           (if A_eq_dec a a' then decode2 rest env' else None)) P.
 Proof.
   unfold cache_inv_Property in *; split.
-  { intros env env' xenv data bin ext env_pm pred_pm com_pf.
+  { intros env env' xenv data bin ext env_pm pred_pm pred_pm_rest com_pf.
     unfold compose, Bind2 in com_pf; computes_to_inv; destruct v;
       destruct v0.
-    destruct (proj1 (decode1_pf (proj1 P_inv_pf)) _ _ _ _ _ (transform b0 ext) env_pm predicate_a' com_pf); intuition; simpl in *; injections.
+    destruct (fun H => proj1 (decode1_pf (proj1 P_inv_pf)) _ _ _ _ _ (transform b0 ext) env_pm predicate_a' H com_pf); intuition; simpl in *; injections.
+    eapply predicate_rest_impl; eauto.
     setoid_rewrite <- transform_assoc; rewrite H2.
     simpl.
     destruct (A_eq_dec a' a'); try congruence.
     subst.
-    destruct (proj1 H5 (*decode2_pf _ (conj (eq_refl _) predicate_a') H1*)
-                    _ _ _ _ _ ext H3 pred_pm com_pf');
+    destruct (fun H => proj1 H5 (*decode2_pf _ (conj (eq_refl _) predicate_a') H1*)
+                    _ _ _ _ _ ext H3 pred_pm H com_pf');
       intuition; simpl in *; injections.
     eauto. }
   { intros.
