src/BinEncoders/Env/Lib2/FixStringOpt.v
@@ -49,10 +49,11 @@ Section String.
       encode_decode_correct_f
         cache transformer
         (fun ls => length ls = sz)
+        (fun _ _ => True)
         encode_string_Spec (decode_string sz) P.
   Proof.
     split.
-    { intros env env' xenv l l' ext Eeq Ppred Penc.
+    { intros env env' xenv l l' ext Eeq Ppred Ppred_rest Penc.
       subst.
       generalize dependent env.
       revert env' xenv l'.
@@ -65,7 +66,7 @@ Section String.
         unfold Bind2 in *; computes_to_inv; subst.
         injection Penc''; intros; subst.
         destruct v; destruct v0.
-        destruct (proj1 (Ascii_decode_correct P_OK) _ _ _ _ _ (transform b0 ext) Eeq I Penc) as [? [? ?] ].
+        destruct (proj1 (Ascii_decode_correct P_OK) _ _ _ _ _ (transform b0 ext) Eeq I I Penc) as [? [? ?] ].
       simpl. rewrite <- transform_assoc, H; simpl.
       destruct (IHl _ _ _ _ H0 Penc') as [? [? ?] ].
       rewrite H1; simpl; eexists; eauto.
